add files

Correctness.v
@@ -15,298 +15,42 @@ Require Import Heap.
 Require Import Effects.
 Require Import Environment.
 Require Import TypeSystem.
+Require Import Determinism.
 Require Import Definitions2.
+Require Import CorrectnessLemmas.
 
 Import TypeSoundness.
 
 
+Definition isPrime := Bool true.
+Definition rho_var := Rgn2_FVar true false "r"%char.
+Definition x_var := "x"%char.
+Definition f := "f"%char.
+Definition rho := "r"%char.
 
-Theorem DynamicDeterminism :
-  forall heap rgns env exp heap1 heap2 val1 val2 acts1 acts2,
-    (heap, rgns, env, exp) ⇓ (heap1, val1, acts1) ->
-    (heap, rgns, env, exp) ⇓ (heap2, val2, acts2) ->
-    (heap1, val1, acts1) = (heap2, val2, acts2).
+Definition incr_body := Cond (isPrime)
+                             (Assign rho_var (Var x_var) (Plus (Const 1) (DeRef rho_var (Var x_var))))
+                             (Assign rho_var (Var x_var) (Var x_var)).
+
+Definition incr_eff := ∅ ⊕ ((∅ ⊕ (∅ ⊕ (ReadConc (Var x_var)))) ⊕ (WriteConc (Var x_var))).
+
+Definition incr_abs := Lambda rho (Mu f x_var (incr_body) (incr_eff)). 
+
+Lemma incr_incr_eff_tfp : BackTriangle2 incr_body incr_eff.
 Proof.
-  intros heap rgns env exp heap1 heap2 val1 val2 acts1 acts2 Dyn1.
-  generalize dependent acts2; generalize dependent val2; generalize dependent heap2.
-  dependent induction Dyn1; intros heap2 val2 acts2 Dyn2; inversion Dyn2; subst;
-  try reflexivity.   
-  - rewrite H in H1. inversion H1. reflexivity.
-  -  assert ( RH1 : (fheap, Cls (env', rho', Mu f x ec' ee'), facts) = (fheap0, Cls (env'0, rho'0, Mu f0 x0 ec'0 ee'0), facts0) )
-      by (eapply IHDyn1_1; [ reflexivity | assumption]); inversion RH1; subst.
-    assert ( RH2 : (aheap, v, aacts) = (aheap0, v0, aacts0) ) by (apply IHDyn1_2; assumption); inversion RH2; subst.
-    assert ( RH3 :  (heap1, val1, bacts) = (heap2, val2, bacts0) ) by (eapply IHDyn1_3; [ reflexivity | reflexivity |  assumption]). 
-    now inversion_clear RH3.
-  (*- assert ( RH1 : (fheap, Cls (env', rho', Mu f x ec' ee'), facts) = (fheap0, Cls (env'0, rho'0, Mu f0 x0 ec'0 ee'0), facts0) )
-      by (eapply IHDyn1_1; [ reflexivity | assumption]); inversion RH1; subst.
-    assert ( RH2 : (aheap, v', aacts) = (aheap0, v, aacts0) ) by (apply IHDyn1_2; assumption); inversion RH2; subst.
-    assert ( RH3 :  (heap1, val1, bacts) = (heap2, val2, bacts0) ).
-    eapply IHDyn1_3; [ reflexivity | reflexivity |  ]. admit.
-    now inversion RH3.*)
-  - assert ( RH1 : (fheap, Cls (env', rho', Lambda x eb), facts) = (fheap0, Cls (env'0, rho'0, Lambda x0 eb0 ), facts0) )
-      by (eapply IHDyn1_1; [ reflexivity | assumption]). inversion RH1; subst.
-    assert ( RH3 :  (heap1, val1, bacts) = (heap2, val2, bacts0) )
-      by (eapply IHDyn1_2; eauto; rewrite H in H9; inversion H9; subst; assumption).
-    now inversion RH3; subst.
-  - assert ( RH1 : (heap2, Cls (env', rho', Mu f x ec' ee'), facts) = (heap2, Cls (env'0, rho'0, Mu f0 x0 ec'0 ee'0), facts0) )
-      by (eapply IHDyn1_1; [ reflexivity | assumption]); inversion RH1; subst.
-    assert ( RH2 : (heap2, v', aacts) = (heap2, v'0, aacts0) ) by (apply IHDyn1_2; assumption); inversion RH2; subst.
-    assert ( RH3 :  (heap2, val1, bacts) = (heap2, val2, bacts0) ) by (eapply IHDyn1_3; [ reflexivity | reflexivity |  assumption]). 
-    now inversion_clear RH3.
-  - admit.  
-  - assert ( RH1 : (cheap, Bit true, cacts) = (cheap0, Bit true, cacts0))
-      by (eapply IHDyn1_1; [ reflexivity | assumption] ); inversion RH1; subst.
-    assert ( RH2 : (heap1, val1, tacts) = (heap2, val2, tacts0)) by (apply IHDyn1_2; assumption).
-    now inversion_clear RH2.
-  - inversion Dyn1_1; inversion H1; subst;
-    repeat (discriminate H12 || discriminate H13 || discriminate H14 || discriminate H15).
-    + inversion H13; subst. rewrite H0 in H10; discriminate H10.
-    + (*assert ( RH1 :(cheap, Bit true, facts0 ++ aacts ++ bacts) = (cheap0, Bit false, facts1 ++ aacts0 ++ bacts0))
-        by (apply IHDyn1_1; [reflexivity | assumption]); now inversion_clear RH1.*)
-      admit.
-    + admit.  
-    + (*assert ( RH1 : (cheap, Bit true, facts0 ++ aacts ++ bacts) = (cheap0, Bit false, facts1 ++ aacts0 ++ bacts0)) 
-        by (apply IHDyn1_1; [reflexivity | assumption]); now inversion_clear RH1.*)
-      admit.
-    + admit.  
-    + (*assert ( RH1 : (cheap, Bit true, cacts1 ++ tacts0) = (cheap0, Bit false, cacts2 ++ facts0)) 
-        by (apply  IHDyn1_1; [reflexivity | assumption]); now inversion_clear RH1.*)
-      admit.
-    + (*assert ( RH1 : (cheap, Bit true, cacts1 ++ facts0) = (cheap0, Bit false, cacts2 ++ tacts0)) 
-        by (apply  IHDyn1_1; [reflexivity | assumption]); now inversion_clear RH1.*)
-      admit.
-    + (*assert ( RH1 : (cheap, Bit true, cacts1 ++ facts0) = (cheap0, Bit false, cacts2 ++ facts1)) 
-        by (apply  IHDyn1_1; [reflexivity | assumption]); now inversion_clear RH1.*)
-      admit.
-    + (*assert ( RH1 : (cheap, Bit true, aacts ++ (DA_Read w l) :: nil) = (cheap0, Bit false, aacts0 ++ (DA_Read w0 l0) :: nil)) 
-        by (apply  IHDyn1_1; [reflexivity | assumption]); now inversion_clear RH1.*)
-      admit.
-    (*+ admit.*)
-    +  assert ( RH1 : (cheap, Bit true, Phi_Seq lacts racts) = (cheap0, Bit false, Phi_Seq lacts0 racts0)) 
-        by (apply  IHDyn1_1; [reflexivity | assumption]); now inversion_clear RH1.
-    (*+ admit.
-    + admit.  *)
-  - assert ( RH1 : (cheap, Bit false, cacts) = (cheap0, Bit true, cacts0) ) 
-        by (apply IHDyn1_1; [reflexivity | assumption]); now inversion_clear RH1.
-  - assert ( RH1 : (cheap, Bit false, cacts) = (cheap0, Bit false, cacts0) )
-      by (apply IHDyn1_1; [reflexivity | assumption]). inversion RH1; subst.
-    assert ( RH2 : (heap1, val1, facts) = (heap2, val2, facts0) )
-      by (apply IHDyn1_2; assumption); now inversion_clear RH2.
-  - assert ( RH1 : (heap', v, vacts) = (heap'0, v0, vacts0) ). 
-    apply IHDyn1. assumption. inversion RH1; subst.
-    rewrite <- H11 in H0. rewrite H in H10. inversion H10; subst.    
-    (* new labels are always picked in some deterministic order, ex. next ascci available *)
-    assert (DetAddr : eq l l0) by admit. 
-    now inversion_clear DetAddr.
-  - assert ( RH1 : (heap1, Loc w l, aacts) = (heap2, Loc w l0, aacts0))
-      by (apply IHDyn1; [reflexivity | assumption]); inversion RH1; subst.
-    rewrite H in H10. inversion H10; subst.
-    rewrite H11 in H0. now inversion_clear H0.
-  - assert ( RH1 : (heap', Loc w l, aacts) = (heap'0, Loc w l0, aacts0))
-      by (apply IHDyn1_1 ; [reflexivity | assumption]); inversion RH1; subst.
-    assert ( RH2 : (heap'', v, vacts) = (heap''0, v0, vacts0))
-      by (apply IHDyn1_2; assumption).
-    rewrite H11 in H. inversion H; subst.
-    now inversion_clear RH2.
-  - assert ( RH1 : (lheap, Num va, lacts) = (lheap0, Num va0, lacts0) )
-      by (apply IHDyn1_1 ;  [reflexivity | assumption]); inversion RH1; subst.
-    assert ( RH2 :  (heap1, Num vb, racts) = (heap2, Num vb0, racts0))
-      by (apply IHDyn1_2;  [reflexivity | assumption]); now inversion_clear RH2.
-  - assert ( RH1 : (lheap, Num va, lacts) = (lheap0, Num va0, lacts0) )
-      by (apply IHDyn1_1 ;  [reflexivity | assumption]); inversion RH1; subst.
-    assert ( RH2 :  (heap1, Num vb, racts) = (heap2, Num vb0, racts0))
-      by (apply IHDyn1_2;  [reflexivity | assumption]); now inversion_clear RH2.
-  - assert ( RH1 : (lheap, Num va, lacts) = (lheap0, Num va0, lacts0) )
-      by (apply IHDyn1_1 ;  [reflexivity | assumption]); inversion RH1; subst.
-    assert ( RH2 :  (heap1, Num vb, racts) = (heap2, Num vb0, racts0))
-      by (apply IHDyn1_2;  [reflexivity | assumption]); now inversion_clear RH2.
-  -  assert ( RH1 : (lheap, Num va, lacts) = (lheap0, Num va0, lacts0) )
-      by (apply IHDyn1_1 ;  [reflexivity | assumption]); inversion RH1; subst.
-    assert ( RH2 :  (heap1, Num vb, racts) = (heap2, Num vb0, racts0))
-       by (apply IHDyn1_2;  [reflexivity | assumption]); now inversion_clear RH2.
-  - (*assert ( RH1 : (heap1, Loc (Rgn_Const r) l, nil) = (heap2, Loc (Rgn_Const r) l0, @nil DynamicAction)).
-    apply IHDyn1. reflexivity. assumption. now inversion RH1; subst.*)
-    admit.
-  - (*assert ( RH1 : (heap1, Loc (Rgn_Const r) l, nil) = (heap2, Loc (Rgn_Const r) l0, @nil DynamicAction)).
-    apply IHDyn1. reflexivity. assumption. now inversion RH1; subst.    *)
-    admit.
-  - (*assert ( RH1 : (heap2, Eff effa, @nil DynamicAction) = (heap2, Eff effa0, nil))
-      by (apply IHDyn1_1 ; [reflexivity | assumption]); inversion RH1; subst.
-     assert ( RH2 : (heap2, Eff effb, @nil DynamicAction) = (heap2, Eff effb0, nil))
-      by (apply IHDyn1_2 ; [reflexivity | assumption]); inversion RH2; subst; reflexivity.*)
-    admit.
-  - admit.
-  - admit.
-  - admit.
-  (*- admit.
-  - admit. *)
-Qed.
-
-Lemma EmptyUnionIsIdentity : 
-  forall p eff, p ⊑ (Union_Theta (Some empty_set) eff) -> p ⊑ eff. 
-Proof.
-  intros p eff H; inversion H; subst; try apply PTS_Nil.  
-  induction eff; apply PTS_Elem;
-  try assert ( HUnionEmpty : (Union_Theta (Some empty_set)  (Some a)) = Some a) 
-     by (unfold Union_Theta, set_union, empty_set; f_equal;
-         apply Extensionality_Ensembles; red; split; unfold Included;
-         intros x Hx; [ inversion Hx; subst; [contradiction | assumption] | apply Union_intror]; auto).
-  - rewrite HUnionEmpty in H0; assumption.
-  - apply DAT_Top. 
-  - induction eff. assert ( HUnionEmpty : (Union_Theta (Some empty_set)  (Some a)) = Some a) 
-     by (unfold Union_Theta, set_union, empty_set; f_equal;
-         apply Extensionality_Ensembles; red; split; unfold Included;
-         intros x Hx; [ inversion Hx; subst; [contradiction | assumption] | apply Union_intror]; auto).
-    rewrite <- HUnionEmpty. auto. now simpl in H.
-  - induction eff. assert ( HUnionEmpty : (Union_Theta (Some empty_set)  (Some a)) = Some a) 
-     by (unfold Union_Theta, set_union, empty_set; f_equal;
-         apply Extensionality_Ensembles; red; split; unfold Included;
-         intros x Hx; [ inversion Hx; subst; [contradiction | assumption] | apply Union_intror]; auto).
-    rewrite <- HUnionEmpty. auto. now simpl in H. 
-Qed.
-
-Definition Correctness_Z :
-  forall stty ctxt rgns ea ee,
-    BackTriangle (stty, ctxt, rgns, ea, ee) ->
-    forall h h' h'' env rho p p' v eff ty static,
-      (h, env, rho, ea) ⇓ (h', v, p) ->
-      (h, env, rho, ee) ⇓ (h'', Eff eff, p') ->
-      ReadOnlyPhi p' ->
-      TcHeap (h, stty) ->
-      TcRho (rho, rgns) ->
-      TcEnv (stty, rho, env, ctxt) -> 
-      TcExp (stty, ctxt, rgns, ea, ty, static) ->    
-      p ⊑ eff.
-Proof.
-  intros stty ctxt rgns ea ee BT.
-  dependent induction BT; intros.
-  - inversion H0; subst.
-    apply PTS_Nil.
-  - inversion H0; subst.
-    apply PTS_Nil.
-  - inversion H0; subst.
-    apply PTS_Nil.
-  - inversion H; subst.
-    apply PTS_Nil.
-  - admit.
-  - inversion H8; subst.
-    inversion H2; subst.
-
-    (*assert (clsTcVal : exists stty',  
-             (forall l t', ST.find l stty = Some t' -> ST.find l stty' = Some t')
-               /\ TcHeap (fheap, stty')
-               /\ TcVal (stty', Cls (env', rho', Mu f0 x0 ec' ee'), subst_rho rho (Ty2_Arrow tya effc ty effe Ty2_Effect))) 
-        by (eapply ty_sound; eauto).
-    destruct clsTcVal as [sttyb [Weakb [TcHeapb TcVal_cls]]]; eauto.
-   
-    assert (argTcVal : exists stty',
-             (forall l t', ST.find l sttyb = Some t' -> ST.find l stty' = Some t')
-               /\ TcHeap (aheap, stty')
-               /\ TcVal (stty', v0, subst_rho rho tya))
-        by (eapply ty_sound; eauto using update_env, ext_stores__env, ext_stores__exp).
-      destruct argTcVal as [sttya [Weaka [TcHeapa TcVal_v']]]; eauto.
-
-      
-      inversion TcVal_cls as  [ | | | ? ? ? ? ? ? ? TcRho_rho' TcEnv_env' TcExp_abs | | ]; subst. 
-      inversion TcExp_abs as [ | | | | ? ? ? ? ? ? ? ? ? TcExp_eb | | | | | | | |  | | | | | | | | | | |  ]; subst.
-      rewrite <- H16 in TcVal_cls.
-      do 2 rewrite subst_rho_arrow in H16. inversion H16. 
-      rewrite <- H10 in TcVal_v'.  *)
-
-      assert (aacts ⊑ Some empty_set).
-      eapply IHBT2 with (ee:=∅) (p':=Phi_Nil); eauto. constructor. constructor.
-      assert (h=fheap) by admit.
-      subst. assumption. 
-      apply EmptyIsNil in H9; subst.
-
-    apply PTS_Seq.
-    + apply PTS_Seq; [| apply PTS_Nil].
-      inversion H13; subst. constructor. 
-    + admit.
-Admitted.
-
-(*Definition Correctness_1 (ea : Expr) (ee : Expr) :
-  forall (h h' h'' : Heap) (env : Env) (rho : Rho) (p p' : Phi) (v : Val) (eff : Theta),
-    (h, env, rho, ea) ⇓ (h', v, p) -> 
-    ReadOnlyPhi p' ->
-    (h, env, rho, ee) ⇓ (h'', Eff eff, p') -> 
-    forall stty ctxt rgns ty static,
-      TcEnv (stty, rho, env, ctxt) -> 
-      TcExp (stty, ctxt, rgns, ea, ty, static) ->    
-      TcHeap (h, stty) ->
-      TcRho (rho, rgns) ->
-      (* BackTriangle (stty, ctxt, rgns, ea, ee) -> p ⊑ eff. *)
-      (ea ◀ ee) -> p ⊑ eff.
-Proof.
-  intros h h' h'' env rho p p' v eff Exprs.
-  generalize dependent eff.
-  generalize dependent p'.
-  generalize dependent ee.
-  dependent induction Exprs;
-  intros edesc p' eff HReadOnly Specs stty ctxt rgns ty static Henv Hexp Hheap HRho Back;
-  inversion Specs; subst; inversion Back; inversion Hexp; subst; try (solve [apply PTS_Nil | apply PhiInThetaTop]).
-  - apply PTS_Seq.      
-    + apply EnsembleUnionComp. 
-      * assert (facts ⊑ effa).
-        eapply IHExprs1 with (ee:=a) (p':=phia); eauto. inversion HReadOnly; auto. assumption.
-      * inversion H7; subst.
-        inversion HReadOnly; subst. inversion H6; subst.
-        assert (aacts ⊑ effa2). 
-        eapply IHExprs2 with (ee:=effa0) (p':=phia0); eauto;
-        assert (ReadOnlyPhi facts) by admit;
-        assert (h''=fheap) by (eapply ReadOnlyTracePreservesHeap_1; eauto); now rewrite <- H0.
-        apply Theta_introl. assumption.
-    + inversion H7; subst.
-      inversion HReadOnly; subst. inversion H6; subst.
-      apply Theta_intror. apply Theta_intror.
-
-      assert (clsTcVal : exists stty',  
-             (forall l t', ST.find l stty = Some t' -> ST.find l stty' = Some t')
-               /\ TcHeap (fheap, stty')
-               /\ TcVal (stty', Cls (env', rho', Mu f x ec' ee'), subst_rho rho (Ty2_Arrow tya effc ty effe Ty2_Effect))) 
-        by (eapply ty_sound; eauto).
-      destruct clsTcVal as [sttyb [Weakb [TcHeapb TcVal_cls]]]; eauto.
-
-      assert (argTcVal : exists stty',
-             (forall l t', ST.find l sttyb = Some t' -> ST.find l stty' = Some t')
-               /\ TcHeap (aheap, stty')
-               /\ TcVal (stty', v0, subst_rho rho tya))
-        by (eapply ty_sound; eauto using update_env, ext_stores__env, ext_stores__exp).
-      destruct argTcVal as [sttya [Weaka [TcHeapa TcVal_v']]]; eauto.
-
-      
-      inversion TcVal_cls as  [ | | | ? ? ? ? ? ? ? TcRho_rho' TcEnv_env' TcExp_abs | | ]; subst. 
-      inversion TcExp_abs as [ | | | | ? ? ? ? ? ? ? ? ? TcExp_eb | | | | | | | |  | | | | | | | | | | |  ]; subst.
-      rewrite <- H16 in TcVal_cls.
-      do 2 rewrite subst_rho_arrow in H16. inversion H16. 
-      rewrite <- H0 in TcVal_v'. 
-      
-      eapply IHExprs3 with (stty := sttya);eauto.
-      * admit.
-      * apply update_env; simpl.
-        eapply ext_stores__env; eauto.
-        { apply update_env; eauto. }
-        { eassumption. }
-      * eapply ext_stores__exp; eauto.
-  - admit. 
-  - admit.
-  - admit.
-(*  - assert ( Hd : (cheap0, Bit false, cacts0) = (cheap, Bit false, cacts)).
-    eapply DynamicDeterminism; eauto; inversion Hd; subst.
-
-    assert (cacts ⊑ Some empty_set). eapply IHExprs1 with (ee:=∅) (p':=Phi_Nil); eauto. constructor.
-    assert (h = h'') by (eapply ReadOnlyTracePreservesHeap_1; eauto); subst. constructor.
-    apply EmptyIsNil in H; subst.
-    apply PTS_Seq; [apply PTS_Nil |].
-    eapply IHExprs2 with (ee:=ef0) (p':=facts0); eauto. 
-    + inversion HReadOnly; auto.
-    + assert (h=cheap0) by (eapply ReadOnlyTracePreservesHeap_1; eauto; inversion HReadOnly; auto); subst.
-      inversion Hd; subst. assumption.
-    + assert (h=cheap0) by (eapply ReadOnlyTracePreservesHeap_1; eauto; inversion HReadOnly; auto); subst.
-      inversion Hd; subst. assumption.
-  - *)
-Admitted.        
-*)
+  unfold incr_body, incr_eff.
+  apply Cond_Cond_2.
+  - apply Bool_Pure.
+  - apply Ref_Write_Conc.
+    + apply Var_Pure.
+    + apply Plus_Concat.
+      * apply Num_Pure.
+      * apply Ref_Read_Conc.
+        { apply Var_Pure. }
+  - apply Ref_Write_Conc.
+    + apply Var_Pure.
+    + apply Var_Pure. 
+Qed. 
 
 Definition Correctness_2 (ea : Expr) (ee : Expr) :
   forall (h h' h'' : Heap) (env : Env) (rho : Rho) (p p' : Phi) (v : Val) (eff : Theta),
@@ -317,7 +61,7 @@ Definition Correctness_2 (ea : Expr) (ee : Expr) :
       TcExp (stty, ctxt, rgns, ea, ty, static) ->    
       TcHeap (h, stty) ->
       TcRho (rho, rgns) ->
-      (ea ◀ ee) -> p ⊑ eff.
+      (BackTriangle2 ea ee) -> p ⊑ eff.
 Proof.
   intros h h' h'' env rho p p' v eff Exprs.
   generalize dependent eff.
@@ -340,7 +84,7 @@ Proof.
       assert (clsTcVal : exists stty',  
              (forall l t', ST.find l stty = Some t' -> ST.find l stty' = Some t')
                /\ TcHeap (fheap, stty')
-               /\ TcVal (stty', Cls (env', rho', Mu f x ec' ee'), subst_rho rho (Ty2_Arrow tya effc ty effe Ty2_Effect))) 
+               /\ TcVal (stty', Cls (env', rho', Mu f0 x ec' ee'), subst_rho rho (Ty2_Arrow tya effc ty effe Ty2_Effect))) 
         by (eapply ty_sound; eauto).
       destruct clsTcVal as [sttyb [Weakb [TcHeapb TcVal_cls]]]; eauto.
 
@@ -376,7 +120,7 @@ Proof.
       assert (clsTcVal : exists stty',  
              (forall l t', ST.find l stty = Some t' -> ST.find l stty' = Some t')
                /\ TcHeap (fheap, stty')
-               /\ TcVal (stty', Cls (env', rho', Mu f x ec' ee'), subst_rho rho (Ty2_Arrow tya effc ty effe Ty2_Effect))) 
+               /\ TcVal (stty', Cls (env', rho', Mu f0 x ec' ee'), subst_rho rho (Ty2_Arrow tya effc ty effe Ty2_Effect))) 
         by (eapply ty_sound; eauto).
       destruct clsTcVal as [sttyb [Weakb [TcHeapb TcVal_cls]]]; eauto.
 
@@ -412,7 +156,7 @@ Proof.
       assert (clsTcVal : exists stty',  
              (forall l t', ST.find l stty = Some t' -> ST.find l stty' = Some t')
                /\ TcHeap (fheap, stty')
-               /\ TcVal (stty', Cls (env', rho', Mu f x ec' ee'), subst_rho rho (Ty2_Arrow tya effc ty effe Ty2_Effect))) 
+               /\ TcVal (stty', Cls (env', rho', Mu f0 x ec' ee'), subst_rho rho (Ty2_Arrow tya effc ty effe Ty2_Effect))) 
         by (eapply ty_sound; eauto).
       destruct clsTcVal as [sttyb [Weakb [TcHeapb TcVal_cls]]]; eauto.
 
@@ -448,7 +192,7 @@ Proof.
       assert (clsTcVal : exists stty',  
              (forall l t', ST.find l stty = Some t' -> ST.find l stty' = Some t')
                /\ TcHeap (fheap, stty')
-               /\ TcVal (stty', Cls (env', rho', Mu f x ec' ee'), subst_rho rho (Ty2_Arrow tya effc ty effe Ty2_Effect))) 
+               /\ TcVal (stty', Cls (env', rho', Mu f0 x ec' ee'), subst_rho rho (Ty2_Arrow tya effc ty effe Ty2_Effect))) 
         by (eapply ty_sound; eauto).
       destruct clsTcVal as [sttyb [Weakb [TcHeapb TcVal_cls]]]; eauto.
 
@@ -484,7 +228,7 @@ Proof.
       assert (clsTcVal : exists stty',  
              (forall l t', ST.find l stty = Some t' -> ST.find l stty' = Some t')
                /\ TcHeap (fheap, stty')
-               /\ TcVal (stty', Cls (env', rho', Mu f x ec' ee'), subst_rho rho (Ty2_Arrow tya effc ty effe Ty2_Effect))) 
+               /\ TcVal (stty', Cls (env', rho', Mu f0 x ec' ee'), subst_rho rho (Ty2_Arrow tya effc ty effe Ty2_Effect))) 
         by (eapply ty_sound; eauto).
       destruct clsTcVal as [sttyb [Weakb [TcHeapb TcVal_cls]]]; eauto.
 
@@ -520,7 +264,7 @@ Proof.
       assert (clsTcVal : exists stty',  
              (forall l t', ST.find l stty = Some t' -> ST.find l stty' = Some t')
                /\ TcHeap (fheap, stty')
-               /\ TcVal (stty', Cls (env', rho', Mu f x ec' ee'), subst_rho rho (Ty2_Arrow tya effc ty effe Ty2_Effect))) 
+               /\ TcVal (stty', Cls (env', rho', Mu f0 x ec' ee'), subst_rho rho (Ty2_Arrow tya effc ty effe Ty2_Effect))) 
         by (eapply ty_sound; eauto).
       destruct clsTcVal as [sttyb [Weakb [TcHeapb TcVal_cls]]]; eauto.
 
@@ -556,7 +300,7 @@ Proof.
       assert (clsTcVal : exists stty',  
              (forall l t', ST.find l stty = Some t' -> ST.find l stty' = Some t')
                /\ TcHeap (fheap, stty')
-               /\ TcVal (stty', Cls (env', rho', Mu f x ec' ee'), subst_rho rho (Ty2_Arrow tya effc ty effe Ty2_Effect))) 
+               /\ TcVal (stty', Cls (env', rho', Mu f0 x ec' ee'), subst_rho rho (Ty2_Arrow tya effc ty effe Ty2_Effect))) 
         by (eapply ty_sound; eauto).
       destruct clsTcVal as [sttyb [Weakb [TcHeapb TcVal_cls]]]; eauto.
 
@@ -592,7 +336,7 @@ Proof.
       assert (clsTcVal : exists stty',  
              (forall l t', ST.find l stty = Some t' -> ST.find l stty' = Some t')
                /\ TcHeap (fheap, stty')
-               /\ TcVal (stty', Cls (env', rho', Mu f x ec' ee'), subst_rho rho (Ty2_Arrow tya effc ty effe Ty2_Effect))) 
+               /\ TcVal (stty', Cls (env', rho', Mu f0 x ec' ee'), subst_rho rho (Ty2_Arrow tya effc ty effe Ty2_Effect))) 
         by (eapply ty_sound; eauto).
       destruct clsTcVal as [sttyb [Weakb [TcHeapb TcVal_cls]]]; eauto.
 
@@ -628,7 +372,7 @@ Proof.
       assert (clsTcVal : exists stty',  
              (forall l t', ST.find l stty = Some t' -> ST.find l stty' = Some t')
                /\ TcHeap (fheap, stty')
-               /\ TcVal (stty', Cls (env', rho', Mu f x ec' ee'), subst_rho rho (Ty2_Arrow tya effc ty effe Ty2_Effect))) 
+               /\ TcVal (stty', Cls (env', rho', Mu f0 x ec' ee'), subst_rho rho (Ty2_Arrow tya effc ty effe Ty2_Effect))) 
         by (eapply ty_sound; eauto).
       destruct clsTcVal as [sttyb [Weakb [TcHeapb TcVal_cls]]]; eauto.
 
@@ -664,7 +408,7 @@ Proof.
       assert (clsTcVal : exists stty',  
              (forall l t', ST.find l stty = Some t' -> ST.find l stty' = Some t')
                /\ TcHeap (fheap, stty')
-               /\ TcVal (stty', Cls (env', rho', Mu f x ec' ee'), subst_rho rho (Ty2_Arrow tya effc ty effe Ty2_Effect))) 
+               /\ TcVal (stty', Cls (env', rho', Mu f0 x ec' ee'), subst_rho rho (Ty2_Arrow tya effc ty effe Ty2_Effect))) 
         by (eapply ty_sound; eauto).
       destruct clsTcVal as [sttyb [Weakb [TcHeapb TcVal_cls]]]; eauto.
 
@@ -700,7 +444,7 @@ Proof.
       assert (clsTcVal : exists stty',  
              (forall l t', ST.find l stty = Some t' -> ST.find l stty' = Some t')
                /\ TcHeap (fheap, stty')
-               /\ TcVal (stty', Cls (env', rho', Mu f x ec' ee'), subst_rho rho (Ty2_Arrow tya effc ty effe Ty2_Effect))) 
+               /\ TcVal (stty', Cls (env', rho', Mu f0 x ec' ee'), subst_rho rho (Ty2_Arrow tya effc ty effe Ty2_Effect))) 
         by (eapply ty_sound; eauto).
       destruct clsTcVal as [sttyb [Weakb [TcHeapb TcVal_cls]]]; eauto.
 
@@ -736,7 +480,7 @@ Proof.
       assert (clsTcVal : exists stty',  
              (forall l t', ST.find l stty = Some t' -> ST.find l stty' = Some t')
                /\ TcHeap (fheap, stty')
-               /\ TcVal (stty', Cls (env', rho', Mu f x ec' ee'), subst_rho rho (Ty2_Arrow tya effc ty effe Ty2_Effect))) 
+               /\ TcVal (stty', Cls (env', rho', Mu f0 x ec' ee'), subst_rho rho (Ty2_Arrow tya effc ty effe Ty2_Effect))) 
         by (eapply ty_sound; eauto).
       destruct clsTcVal as [sttyb [Weakb [TcHeapb TcVal_cls]]]; eauto.
 
@@ -772,7 +516,7 @@ Proof.
       assert (clsTcVal : exists stty',  
              (forall l t', ST.find l stty = Some t' -> ST.find l stty' = Some t')
                /\ TcHeap (fheap, stty')
-               /\ TcVal (stty', Cls (env', rho', Mu f x ec' ee'), subst_rho rho (Ty2_Arrow tya effc ty effe Ty2_Effect))) 
+               /\ TcVal (stty', Cls (env', rho', Mu f0 x ec' ee'), subst_rho rho (Ty2_Arrow tya effc ty effe Ty2_Effect))) 
         by (eapply ty_sound; eauto).
       destruct clsTcVal as [sttyb [Weakb [TcHeapb TcVal_cls]]]; eauto.
 
@@ -808,7 +552,7 @@ Proof.
       assert (clsTcVal : exists stty',  
              (forall l t', ST.find l stty = Some t' -> ST.find l stty' = Some t')
                /\ TcHeap (fheap, stty')
-               /\ TcVal (stty', Cls (env', rho', Mu f x ec' ee'), subst_rho rho (Ty2_Arrow tya effc ty effe Ty2_Effect))) 
+               /\ TcVal (stty', Cls (env', rho', Mu f0 x ec' ee'), subst_rho rho (Ty2_Arrow tya effc ty effe Ty2_Effect))) 
         by (eapply ty_sound; eauto).
       destruct clsTcVal as [sttyb [Weakb [TcHeapb TcVal_cls]]]; eauto.
 
@@ -844,7 +588,7 @@ Proof.
       assert (clsTcVal : exists stty',  
              (forall l t', ST.find l stty = Some t' -> ST.find l stty' = Some t')
                /\ TcHeap (fheap, stty')
-               /\ TcVal (stty', Cls (env', rho', Mu f x ec' ee'), subst_rho rho (Ty2_Arrow tya effc ty effe Ty2_Effect))) 
+               /\ TcVal (stty', Cls (env', rho', Mu f0 x ec' ee'), subst_rho rho (Ty2_Arrow tya effc ty effe Ty2_Effect))) 
         by (eapply ty_sound; eauto).
       destruct clsTcVal as [sttyb [Weakb [TcHeapb TcVal_cls]]]; eauto.
 
@@ -880,7 +624,7 @@ Proof.
       assert (clsTcVal : exists stty',  
              (forall l t', ST.find l stty = Some t' -> ST.find l stty' = Some t')
                /\ TcHeap (fheap, stty')
-               /\ TcVal (stty', Cls (env', rho', Mu f x ec' ee'), subst_rho rho (Ty2_Arrow tya effc ty effe Ty2_Effect))) 
+               /\ TcVal (stty', Cls (env', rho', Mu f0 x ec' ee'), subst_rho rho (Ty2_Arrow tya effc ty effe Ty2_Effect))) 
         by (eapply ty_sound; eauto).
       destruct clsTcVal as [sttyb [Weakb [TcHeapb TcVal_cls]]]; eauto.
 
@@ -916,7 +660,7 @@ Proof.
       assert (clsTcVal : exists stty',  
              (forall l t', ST.find l stty = Some t' -> ST.find l stty' = Some t')
                /\ TcHeap (fheap, stty')
-               /\ TcVal (stty', Cls (env', rho', Mu f x ec' ee'), subst_rho rho (Ty2_Arrow tya effc ty effe Ty2_Effect))) 
+               /\ TcVal (stty', Cls (env', rho', Mu f0 x ec' ee'), subst_rho rho (Ty2_Arrow tya effc ty effe Ty2_Effect))) 
         by (eapply ty_sound; eauto).
       destruct clsTcVal as [sttyb [Weakb [TcHeapb TcVal_cls]]]; eauto.
 
@@ -952,7 +696,7 @@ Proof.
       assert (clsTcVal : exists stty',  
              (forall l t', ST.find l stty = Some t' -> ST.find l stty' = Some t')
                /\ TcHeap (fheap, stty')
-               /\ TcVal (stty', Cls (env', rho', Mu f x ec' ee'), subst_rho rho (Ty2_Arrow tya effc ty effe Ty2_Effect))) 
+               /\ TcVal (stty', Cls (env', rho', Mu f0 x ec' ee'), subst_rho rho (Ty2_Arrow tya effc ty effe Ty2_Effect))) 
         by (eapply ty_sound; eauto).
       destruct clsTcVal as [sttyb [Weakb [TcHeapb TcVal_cls]]]; eauto.
 
@@ -988,7 +732,7 @@ Proof.
       assert (clsTcVal : exists stty',  
              (forall l t', ST.find l stty = Some t' -> ST.find l stty' = Some t')
                /\ TcHeap (fheap, stty')
-               /\ TcVal (stty', Cls (env', rho', Mu f x ec' ee'), subst_rho rho (Ty2_Arrow tya effc ty effe Ty2_Effect))) 
+               /\ TcVal (stty', Cls (env', rho', Mu f0 x ec' ee'), subst_rho rho (Ty2_Arrow tya effc ty effe Ty2_Effect))) 
         by (eapply ty_sound; eauto).
       destruct clsTcVal as [sttyb [Weakb [TcHeapb TcVal_cls]]]; eauto.
 
@@ -1024,7 +768,7 @@ Proof.
       assert (clsTcVal : exists stty',  
              (forall l t', ST.find l stty = Some t' -> ST.find l stty' = Some t')
                /\ TcHeap (fheap, stty')
-               /\ TcVal (stty', Cls (env', rho', Mu f x ec' ee'), subst_rho rho (Ty2_Arrow tya effc ty effe Ty2_Effect))) 
+               /\ TcVal (stty', Cls (env', rho', Mu f0 x ec' ee'), subst_rho rho (Ty2_Arrow tya effc ty effe Ty2_Effect))) 
         by (eapply ty_sound; eauto).
       destruct clsTcVal as [sttyb [Weakb [TcHeapb TcVal_cls]]]; eauto.
 
@@ -1060,7 +804,7 @@ Proof.
       assert (clsTcVal : exists stty',  
              (forall l t', ST.find l stty = Some t' -> ST.find l stty' = Some t')
                /\ TcHeap (fheap, stty')
-               /\ TcVal (stty', Cls (env', rho', Mu f x ec' ee'), subst_rho rho (Ty2_Arrow tya effc ty effe Ty2_Effect))) 
+               /\ TcVal (stty', Cls (env', rho', Mu f0 x ec' ee'), subst_rho rho (Ty2_Arrow tya effc ty effe Ty2_Effect))) 
         by (eapply ty_sound; eauto).
       destruct clsTcVal as [sttyb [Weakb [TcHeapb TcVal_cls]]]; eauto.
 
@@ -1096,7 +840,7 @@ Proof.
       assert (clsTcVal : exists stty',  
              (forall l t', ST.find l stty = Some t' -> ST.find l stty' = Some t')
                /\ TcHeap (fheap, stty')
-               /\ TcVal (stty', Cls (env', rho', Mu f x ec' ee'), subst_rho rho (Ty2_Arrow tya effc ty effe Ty2_Effect))) 
+               /\ TcVal (stty', Cls (env', rho', Mu f0 x ec' ee'), subst_rho rho (Ty2_Arrow tya effc ty effe Ty2_Effect))) 
         by (eapply ty_sound; eauto).
       destruct clsTcVal as [sttyb [Weakb [TcHeapb TcVal_cls]]]; eauto.
 
@@ -1132,7 +876,7 @@ Proof.
       assert (clsTcVal : exists stty',  
              (forall l t', ST.find l stty = Some t' -> ST.find l stty' = Some t')
                /\ TcHeap (fheap, stty')
-               /\ TcVal (stty', Cls (env', rho', Mu f x ec' ee'), subst_rho rho (Ty2_Arrow tya effc ty effe Ty2_Effect))) 
+               /\ TcVal (stty', Cls (env', rho', Mu f0 x ec' ee'), subst_rho rho (Ty2_Arrow tya effc ty effe Ty2_Effect))) 
         by (eapply ty_sound; eauto).
       destruct clsTcVal as [sttyb [Weakb [TcHeapb TcVal_cls]]]; eauto.
 
@@ -1168,7 +912,7 @@ Proof.
       assert (clsTcVal : exists stty',  
              (forall l t', ST.find l stty = Some t' -> ST.find l stty' = Some t')
                /\ TcHeap (fheap, stty')
-               /\ TcVal (stty', Cls (env', rho', Mu f x ec' ee'), subst_rho rho (Ty2_Arrow tya effc ty effe Ty2_Effect))) 
+               /\ TcVal (stty', Cls (env', rho', Mu f0 x ec' ee'), subst_rho rho (Ty2_Arrow tya effc ty effe Ty2_Effect))) 
         by (eapply ty_sound; eauto).
       destruct clsTcVal as [sttyb [Weakb [TcHeapb TcVal_cls]]]; eauto.
 
@@ -1207,7 +951,7 @@ Proof.
     +  assert (clsTcVal : exists stty',  
              (forall l t', ST.find l stty = Some t' -> ST.find l stty' = Some t')
                /\ TcHeap (fheap, stty')
-               /\ TcVal (stty', Cls (env', rho', Mu f x ec' ee'), subst_rho rho (Ty2_Arrow tya effc ty effe Ty2_Effect))) 
+               /\ TcVal (stty', Cls (env', rho', Mu f0 x ec' ee'), subst_rho rho (Ty2_Arrow tya effc ty effe Ty2_Effect))) 
         by (eapply ty_sound; eauto).
       destruct clsTcVal as [sttyb [Weakb [TcHeapb TcVal_cls]]]; eauto.
 
@@ -1246,7 +990,7 @@ Proof.
     +  assert (clsTcVal : exists stty',  
              (forall l t', ST.find l stty = Some t' -> ST.find l stty' = Some t')
                /\ TcHeap (fheap, stty')
-               /\ TcVal (stty', Cls (env', rho', Mu f x ec' ee'), subst_rho rho (Ty2_Arrow tya effc ty effe Ty2_Effect))) 
+               /\ TcVal (stty', Cls (env', rho', Mu f0 x ec' ee'), subst_rho rho (Ty2_Arrow tya effc ty effe Ty2_Effect))) 
         by (eapply ty_sound; eauto).
       destruct clsTcVal as [sttyb [Weakb [TcHeapb TcVal_cls]]]; eauto.
 
@@ -1290,7 +1034,7 @@ Proof.
       assert (clsTcVal : exists stty',  
              (forall l t', ST.find l stty = Some t' -> ST.find l stty' = Some t')
                /\ TcHeap (fheap, stty')
-               /\ TcVal (stty', Cls (env', rho', Mu f x ec' ee'), subst_rho rho (Ty2_Arrow tya effc ty effe Ty2_Effect))) 
+               /\ TcVal (stty', Cls (env', rho', Mu f0 x ec' ee'), subst_rho rho (Ty2_Arrow tya effc ty effe Ty2_Effect))) 
         by (eapply ty_sound; eauto).
       destruct clsTcVal as [sttyb [Weakb [TcHeapb TcVal_cls]]]; eauto.
 
