Correctness3.v
@@ -1,0 +1,74 @@
+Require Import Coq.Program.Equality.
+Require Import Coq.Sets.Ensembles.
+Require Import Coq.FSets.FMapAVL. 
+Require Import Coq.Structures.OrderedTypeEx.
+Require Import Coq.Arith.Peano_dec.
+Require Import Ascii String.
+Require Import Coq.Arith.EqNat.
+Require Import Coq.Arith.Mult.
+Require Import Coq.Arith.Plus.
+Require Import Coq.Arith.Minus.
+Require Import Coq.Lists.List.
+Require Import Coq.Arith.Compare_dec.
+Require Import Keys.
+Require Import Heap.
+Require Import Effects.
+Require Import Environment.
+Require Import TypeSystem.
+Require Import Determinism.
+Require Import Definitions2.
+Require Import CorrectnessLemmas.
+
+Import TypeSoundness.
+
+Definition Correctness_Z :
+  forall stty ctxt rgns ea ee,
+    BackTriangle (stty, ctxt, rgns, ea, ee) ->
+    forall h h' h'' env rho p p' v eff ty static,
+      (h, env, rho, ea) ⇓ (h', v, p) ->
+      (h, env, rho, ee) ⇓ (h'', Eff eff, p') ->
+      ReadOnlyPhi p' ->
+      TcHeap (h, stty) ->
+      TcRho (rho, rgns) ->
+      TcEnv (stty, rho, env, ctxt) -> 
+      TcExp (stty, ctxt, rgns, ea, ty, static) ->    
+      p ⊑ eff.
+Proof.
+  intros stty ctxt rgns ea ee BT.
+  dependent induction BT; intros.
+  - inversion H0; subst.
+    apply PTS_Nil.
+  - inversion H0; subst.
+    apply PTS_Nil.
+  - inversion H0; subst.
+    apply PTS_Nil.
+  - inversion H; subst.
+    apply PTS_Nil.
+  - inversion H1; subst.
+    inversion H7; subst.
+    inversion H2; subst.
+
+    assert (clsTcVal : exists stty',  
+             (forall l t', ST.find l stty = Some t' -> ST.find l stty' = Some t')
+               /\ TcHeap (fheap, stty')
+               /\ TcVal (stty', Cls (env', rho', Mu f x ec' ee'), subst_rho rho (Ty2_Arrow tya effc ty effe Ty2_Effect))) 
+        by (eapply ty_sound; eauto).
+    destruct clsTcVal as [sttyb [Weakb [TcHeapb TcVal_cls]]]; eauto.
+   
+    assert (argTcVal : exists stty',
+             (forall l t', ST.find l sttyb = Some t' -> ST.find l stty' = Some t')
+               /\ TcHeap (aheap, stty')
+               /\ TcVal (stty', v0, subst_rho rho tya))
+        by (eapply ty_sound; eauto using update_env, ext_stores__env, ext_stores__exp).
+      destruct argTcVal as [sttya [Weaka [TcHeapa TcVal_v']]]; eauto.
+
+      
+      inversion TcVal_cls as  [ | | | ? ? ? ? ? ? ? TcRho_rho' TcEnv_env' TcExp_abs | | ]; subst. 
+      inversion TcExp_abs as [ | | | | ? ? ? ? ? ? ? ? ? TcExp_eb | | | | | | | |  | | | | | | | | | | |  ]; subst.
+      rewrite <- H16 in TcVal_cls.
+      do 2 rewrite subst_rho_arrow in H16. inversion H16. 
+      rewrite <- H9 in TcVal_v'. 
+
+      assert (facts ⊑ Some empty_set).
+      admit.
+Admitted.
