CorrectnessLemmas.v
@@ -1,0 +1,299 @@
+Require Import Coq.Program.Equality.
+Require Import Coq.Sets.Ensembles.
+Require Import Definitions2.
+
+
+Reserved Notation "phi '⊑' theta" (at level 50, left associativity).
+Inductive Phi_Theta_Soundness : Phi -> Theta -> Prop :=
+| PTS_Nil :
+    forall theta, (Phi_Nil) ⊑ theta
+| PTS_Elem : forall da theta,
+      DA_in_Theta da theta ->
+      (Phi_Elem da) ⊑ theta
+| PTS_Seq : forall phi1 phi2 theta,
+      phi1 ⊑ theta ->
+      phi2 ⊑ theta ->
+      Phi_Seq phi1 phi2 ⊑ theta
+| PTS_Par : forall phi1 phi2 theta,
+      phi1 ⊑ theta ->
+      phi2 ⊑ theta ->
+      Phi_Par phi1 phi2 ⊑ theta
+where "phi '⊑' theta" := (Phi_Theta_Soundness phi theta) : type_scope.
+
+Axiom Phi_Seq_Nil_L : forall phi, Phi_Seq Phi_Nil phi = phi.
+Axiom Phi_Seq_Nil_R : forall phi, Phi_Seq phi Phi_Nil = phi.
+Axiom Phi_Par_Nil_R : forall phi, Phi_Par Phi_Nil phi = phi.
+Axiom Phi_Par_Nil_L : forall phi, Phi_Par Phi_Nil phi = phi.
+
+Lemma PhiInThetaTop:
+  forall phi, phi ⊑ Theta_Top.
+Proof.  
+  induction phi; intros; econstructor; try assumption; apply DAT_Top.
+Qed.
+
+Lemma EmptyIsNil:
+  forall phi, phi ⊑ Theta_Empty -> phi = Phi_Nil.
+Proof.
+  induction phi; intros.
+  reflexivity.
+  inversion H; subst; inversion H1; subst; try (solve [contradiction]).
+  - admit.
+  - admit.  
+  - assert ( H1 : phi1 = Phi_Nil ) by (apply IHphi1; inversion H; assumption); rewrite H1.
+    assert ( H2 : phi2 = Phi_Nil ) by (apply IHphi2; inversion H; assumption); rewrite H2.
+    rewrite Phi_Par_Nil_R. reflexivity.
+  - assert ( H1 : phi1 = Phi_Nil ) by (apply IHphi1; inversion H; assumption); rewrite H1.
+    assert ( H2 : phi2 = Phi_Nil ) by (apply IHphi2; inversion H; assumption); rewrite H2.
+    rewrite Phi_Seq_Nil_R. reflexivity.  
+Qed.
+
+
+Lemma EmptyInAnyTheta:
+  forall phi theta, phi ⊑ Theta_Empty -> phi ⊑ theta .
+Proof.  
+  induction phi; intros; try (solve [econstructor]).
+  - inversion H; subst; inversion H1; subst; inversion H3; subst;
+    try (solve [assert (set_union acts a = empty_set -> acts = empty_set) by admit; apply H2 in H0; subst; inversion H5]);
+    try (solve [admit]).
+  - inversion H; subst. apply EmptyIsNil in H2. apply EmptyIsNil in H4. subst.
+    apply PTS_Par. apply IHphi1. apply PTS_Nil.  apply IHphi1. apply PTS_Nil.
+  - inversion H; subst. apply EmptyIsNil in H2. apply EmptyIsNil in H4. subst.
+    apply PTS_Seq. apply IHphi1. apply PTS_Nil.  apply IHphi1. apply PTS_Nil. 
+ Qed.
+
+Lemma EnsembleUnionSym :
+  forall (phi : Phi) (theta theta' : Theta),
+    phi ⊑ theta -> phi ⊑ (Union_Theta theta theta') /\ phi ⊑ (Union_Theta theta' theta).
+Proof.
+  intros phi theta theta' H.
+  generalize dependent theta'.
+  induction H; intros theta'.
+  - split; [apply PTS_Nil | apply PTS_Nil]. 
+  - destruct theta as [acts|]; destruct theta' as [acts'|]; intuition; simpl;
+    try (apply PTS_Elem; inversion H; subst; apply DAT_Top). 
+    + econstructor. apply DAT_intror. assumption.
+    + econstructor. apply DAT_introl. assumption.
+  - destruct theta as [acts|]; destruct theta' as [acts'|]; intuition;
+    (apply PTS_Seq; [apply IHPhi_Theta_Soundness1 | apply IHPhi_Theta_Soundness2]).
+  - split; destruct theta as [acts|]; destruct theta' as [acts'|]; intuition;
+    (apply PTS_Par; [apply IHPhi_Theta_Soundness1 | apply IHPhi_Theta_Soundness2]).  
+Qed.
+
+Lemma EmptyUnionIsIdentity : 
+  forall p eff, p ⊑ (Union_Theta (Some empty_set) eff) -> p ⊑ eff. 
+Proof.
+  intros p eff H; inversion H; subst; try apply PTS_Nil.  
+  induction eff; apply PTS_Elem;
+  try assert ( HUnionEmpty : (Union_Theta (Some empty_set)  (Some a)) = Some a) 
+     by (unfold Union_Theta, set_union, empty_set; f_equal;
+         apply Extensionality_Ensembles; red; split; unfold Included;
+         intros x Hx; [ inversion Hx; subst; [contradiction | assumption] | apply Union_intror]; auto).
+  - rewrite HUnionEmpty in H0; assumption.
+  - apply DAT_Top. 
+  - induction eff. assert ( HUnionEmpty : (Union_Theta (Some empty_set)  (Some a)) = Some a) 
+     by (unfold Union_Theta, set_union, empty_set; f_equal;
+         apply Extensionality_Ensembles; red; split; unfold Included;
+         intros x Hx; [ inversion Hx; subst; [contradiction | assumption] | apply Union_intror]; auto).
+    rewrite <- HUnionEmpty. auto. now simpl in H.
+  - induction eff. assert ( HUnionEmpty : (Union_Theta (Some empty_set)  (Some a)) = Some a) 
+     by (unfold Union_Theta, set_union, empty_set; f_equal;
+         apply Extensionality_Ensembles; red; split; unfold Included;
+         intros x Hx; [ inversion Hx; subst; [contradiction | assumption] | apply Union_intror]; auto).
+    rewrite <- HUnionEmpty. auto. now simpl in H. 
+Qed.
+
+Lemma EnsembleUnionComp :
+  forall (phi1 phi2 : Phi) (theta1 theta2 : Theta),
+    phi1 ⊑ theta1 -> phi2 ⊑ theta2 -> Phi_Seq phi1  phi2 ⊑ (Union_Theta theta1 theta2).
+Proof. 
+  intros phi1 phi2 theta1 theta2 H1 H2.
+  econstructor.
+  - apply EnsembleUnionSym with (theta' := theta2) in H1. intuition. 
+  - apply EnsembleUnionSym with (theta' := theta1) in H2. intuition.
+Qed.
+
+
+Lemma Theta_introl: 
+  forall phi theta1 theta2, phi ⊑ theta1 -> phi ⊑ Union_Theta theta1 theta2.
+Proof.
+  induction phi; intros; try (solve [econstructor]).
+  - inversion H; subst; inversion H1; subst; simpl;
+    try (solve [assumption |
+                induction theta2; [econstructor; constructor; now apply Union_introl | econstructor; constructor] |
+                induction theta2; [econstructor; now apply DAT_intror | econstructor; constructor ]] ).
+  - apply PTS_Par. apply IHphi1. now inversion H. apply IHphi2. now inversion H.
+  - apply PTS_Seq. apply IHphi1. now inversion H. apply IHphi2. now inversion H.
+Qed.    
+
+Lemma Theta_intror:
+  forall phi theta1 theta2, phi ⊑ theta1 -> phi ⊑ Union_Theta theta2 theta1.
+Proof.
+  induction phi; intros; try (solve [econstructor]).
+  - inversion H; subst; inversion H1; subst; simpl;
+    try (solve [assumption |
+                induction theta2; [econstructor; constructor; now apply Union_intror | econstructor; constructor] |
+                induction theta2; [econstructor; now apply DAT_introl | econstructor; constructor ]] ).
+  - apply PTS_Par. apply IHphi1. now inversion H. apply IHphi2. now inversion H.
+  - apply PTS_Seq. apply IHphi1. now inversion H. apply IHphi2. now inversion H.
+Qed.
+
+Lemma EmptyTracePreservesHeap_1 : 
+  forall h r env e same_h v' acts, (h, r, env, e) ⇓ (same_h, v', acts) -> acts = Phi_Nil -> h = same_h.
+Proof.
+  intros h r env e same_h v' acts H Hnil.  (*destruct H as [H Hnil]. *)
+  dependent induction H; auto; inversion Hnil.
+  - eapply IHBigStep; [reflexivity | auto].
+  - eapply IHBigStep; [reflexivity | auto]. 
+Qed.
+
+Lemma ReadOnlyTracePreservesHeap_1 : 
+  forall h env rho e same_h v' acts, (h, env, rho, e) ⇓ (same_h, v', acts) -> 
+                                   ReadOnlyPhi acts -> h = same_h.
+Proof.
+  intros h env rho e same_h v' acts H.
+  dependent induction H; intros;
+  try (solve [reflexivity]).
+  - inversion H2; inversion H5; subst;
+    assert (h=fheap) by (eapply  IHBigStep1; [reflexivity | assumption]); subst;
+    assert (aheap=fheap) by (symmetry; eapply IHBigStep2; assumption); subst;
+    (eapply IHBigStep3; [reflexivity | reflexivity | assumption]).
+  - inversion H2; subst;
+    assert (h=fheap) by (eapply  IHBigStep1; [reflexivity | assumption]); subst;
+    (eapply IHBigStep2; [reflexivity | reflexivity | assumption]). 
+  - admit.
+  - inversion H1; subst;
+    assert (h=cheap) by (eapply  IHBigStep1; [reflexivity | assumption]); subst;
+    (eapply IHBigStep2; assumption).
+  - inversion H1; subst;
+    assert (h=cheap) by (eapply  IHBigStep1; [reflexivity | assumption]); subst;
+    (eapply IHBigStep2; assumption).
+  - inversion H2; inversion H6.
+  - inversion H2; subst; (eapply IHBigStep; [reflexivity | assumption]).
+  - inversion H2; inversion H6.
+  - inversion H1; subst;
+    assert (h=lheap) by (eapply IHBigStep1; [reflexivity | assumption]); subst;
+    (eapply IHBigStep2; [reflexivity | assumption]).
+  - inversion H1; subst;
+    assert (h=lheap) by (eapply IHBigStep1; [reflexivity | assumption]); subst;
+    (eapply IHBigStep2; [reflexivity | assumption]).
+  - inversion H1; subst;
+    assert (h=lheap) by (eapply IHBigStep1; [reflexivity | assumption]); subst;
+    (eapply IHBigStep2; [reflexivity | assumption]).
+  - inversion H1; subst;
+    assert (h=lheap) by (eapply IHBigStep1; [reflexivity | assumption]); subst;
+    (eapply IHBigStep2; [reflexivity | assumption]).
+  - eapply EmptyTracePreservesHeap_1; eauto.
+  - eapply EmptyTracePreservesHeap_1; eauto.
+Qed.    
+
+Inductive SA_DA_Soundness : StaticAction -> DynamicAction -> Prop :=
+| SA_DA_Read : forall r l, SA_DA_Soundness (SA_Read (Rgn2_Const true true r)) (DA_Read r l)
+| SA_DA_Write : forall r l, SA_DA_Soundness (SA_Write (Rgn2_Const true true r)) (DA_Write r l)
+| SA_DA_Alloc : forall r l, SA_DA_Soundness (SA_Alloc (Rgn2_Const true true r)) (DA_Alloc r l).
+
+Inductive Epsilon_Phi_Soundness :  (Epsilon * Phi) -> Prop := 
+  | EPS : forall st dy, (forall da, DA_in_Phi da dy -> exists sa, Ensembles.In StaticAction st sa /\ SA_DA_Soundness sa da) -> Epsilon_Phi_Soundness (st, dy).
+
+Lemma ReadOnlyStaticImpliesReadOnlySubstStatic : 
+  forall eps rho,
+    ReadOnlyStatic eps ->
+    ReadOnlyStatic (fold_subst_eps rho eps).
+Proof.
+  intros eps rho ROS.
+  induction ROS.
+  - replace (fold_subst_eps rho Empty_Static_Action) with (Empty_Static_Action).
+    constructor.
+    apply Extensionality_Ensembles;
+    unfold Same_set, Included; split; intros x H; unfold Ensembles.In in *.
+    inversion H. inversion H. destruct H0. inversion H0.
+  - replace (fold_subst_eps rho (Singleton_Static_Action (SA_Read r))) with (Singleton_Static_Action (SA_Read (fold_subst_rgn rho r))).
+    constructor.
+    apply Extensionality_Ensembles;
+    unfold Same_set, Included; split; intros x H; unfold Ensembles.In in *.
+    inversion H.
+    unfold fold_subst_eps. exists (SA_Read r). intuition.
+    inversion H. inversion H0. inversion H1. subst. unfold fold_subst_sa; simpl. apply Ensembles.In_singleton.
+  - replace (fold_subst_eps rho (Union_Static_Action eps1 eps2)) with (Union_Static_Action (fold_subst_eps rho eps1) (fold_subst_eps rho eps2)).
+    constructor; assumption.
+    apply Extensionality_Ensembles;
+    unfold Same_set, Included; split; intros x H; unfold Ensembles.In in *.
+    inversion H; subst; inversion H0; unfold fold_subst_eps; exists x0; split;
+    [apply Ensembles.Union_introl | | apply Ensembles.Union_intror | ]; intuition.
+    inversion H. inversion H0. inversion H1; subst;
+    [apply Ensembles.Union_introl | apply Ensembles.Union_intror]; unfold Ensembles.In; unfold fold_subst_eps; exists x0; intuition.
+Qed.
+
+Lemma ReadOnlyStaticImpliesReadOnlyPhi :
+  forall eps phi,
+    ReadOnlyStatic eps ->
+    Epsilon_Phi_Soundness (eps, phi) ->
+    ReadOnlyPhi phi.
+Proof.
+  intros eps phi. induction phi; intros ROS H.
+  - constructor.
+  - induction d.
+    + exfalso; induction ROS.
+      * inversion H; subst. 
+        edestruct H1; [econstructor | destruct H0 ; inversion H0].
+      * inversion H; subst.
+        edestruct H1; [econstructor | destruct H0 ; inversion H0; subst; inversion H2 ].
+      * inversion H; subst. destruct (H1 (DA_Alloc r n)) as [ ? [ ? ? ]]; [ constructor | ].
+        inversion H0; subst.
+        apply IHROS1; constructor; intros; inversion H4; subst; exists x; intuition.
+        apply IHROS2; constructor; intros; inversion H4; subst; exists x; intuition.
+    + econstructor.
+    + exfalso; induction ROS.
+      * inversion H; subst. 
+        edestruct H1; [econstructor | destruct H0 ; inversion H0].
+      * inversion H; subst.
+        edestruct H1; [econstructor | destruct H0 ; inversion H0; subst; inversion H2 ].
+      * inversion H; subst. destruct (H1 (DA_Write r n)) as [ ? [ ? ? ]]; [ constructor | ].
+        inversion H0; subst.
+        apply IHROS1; constructor; intros; inversion H4; subst; exists x; intuition.
+        apply IHROS2; constructor; intros; inversion H4; subst; exists x; intuition.
+  - assert (Epsilon_Phi_Soundness (eps, phi1)).
+    constructor; intros da daIn; inversion H; subst; apply (H1 da); apply DAP_Par; auto.
+    assert (Epsilon_Phi_Soundness (eps, phi2)).
+    constructor; intros da daIn; inversion H; subst; apply (H2 da); apply DAP_Par; auto.
+    constructor; auto.
+  - assert (Epsilon_Phi_Soundness (eps, phi1)).
+    constructor; intros da daIn; inversion H; subst; apply (H1 da); apply DAP_Seq; auto.
+    assert (Epsilon_Phi_Soundness (eps, phi2)).
+    constructor; intros da daIn; inversion H; subst; apply (H2 da); apply DAP_Seq; auto.
+    constructor; auto.
+Qed.
+
+Lemma EmptyTracePreservesHeap_2 : 
+  forall h r env e same_h v acts,
+    (h, r, env, e) ⇓ (h, v, acts) -> h = same_h -> (same_h, r, env, e) ⇓ (same_h, v, acts).
+Proof.
+  intros h r env e same_h v' acts Dyn H. now subst.
+Qed.
+
+Lemma EmptyTracePreservesHeap_3 : 
+  forall h r env e same_h v acts,
+    (same_h, r, env, e) ⇓ (same_h, v, acts) -> (h, r, env, e) ⇓ (same_h, v, acts) -> acts = Phi_Nil -> (h, r, env, e) ⇓ (h, v, acts).
+Proof.
+  intros h r env e same_h v' acts H Dyn1 Hnil.
+  apply EmptyTracePreservesHeap_1 in Dyn1. now subst. exact Hnil.
+Qed.
+
+Lemma EmptyTracePreservesHeap_4 : 
+  forall h r env e same_h v,
+    (h, r, env, e) ⇓ (same_h, v, Phi_Nil) -> h = same_h.
+Proof.
+   intros h r env e same_h v' Dyn1.
+   dependent induction Dyn1; auto.
+   eapply IHDyn1. reflexivity. eapply IHDyn1. reflexivity.
+Qed.
+
+
+Lemma EmptyTracePreservesHeap_5 : 
+  forall h r env e  v,
+    (h, r, env, e) ⇓ (h, v, Phi_Nil) ->
+    exists same_h,  (same_h, r, env, e) ⇓ (h, v, Phi_Nil).
+Proof.
+  intros h r env e v H.
+  dependent induction H; exists h; econstructor; auto.
+  assumption. assumption.
+Qed.
