TypeSystem.v
@@ -9,6 +9,7 @@ Require Import Tactics.
 Require Import Keys.
 Require Import Definitions2.
 Require Import Nameless2.
+Require Import CorrectnessLemmas.
 Require Import Environment.
 Require Import Heap. 
 
